lib/Syntax.v
@@ -1,3 +1,4 @@
 Inductive expr : Type :=
 | ValE : nat -> expr
-| AddE : expr -> expr -> expr.
+| AddE : expr -> expr -> expr
+| SubE : expr -> expr -> expr.
